incr_cas/IncrementIAproof.v
@@ -4,14 +4,16 @@ Require Import ImpPrelude MemHeader MemA.
 From CRIS.incr_cas Require Import Header IncrementI IncrementA.
 
 Module IncrementIA. Section IncrementIA.
-  Context `{!crisG Γ Σ α β τ _S _I, !memG, !schG}.
+  Context `{CrisG: !crisG Γ Σ α β τ _S _I}.
+  Context `{MemG: !memG}.
+  Context `{SchG: !schG}.
 
   Local Definition IstFull := (IstProd (IstSB IncrementA.t.(Mod.scopes) IstTrue) IstEq).
-  Local Definition MA := (IncrementA.t ★ MemP.t).
-  Local Definition MI := (IncrementI.t ★ MemP.t).
+  Local Definition MA := (IncrementA.t ★ MemA.t).
+  Local Definition MI := (IncrementI.t ★ MemA.t).
 
   Lemma increment_simF : ISim.sim_fun open MA MI True%I IstFull (Some IncrementHdr.increment).
-  Proof.
+  Proof using MemG SchG.
     init_simF.
     steps_l. destruct _q; ss. destruct _q; ss. destruct v; ss. inv G0. hss.
     destruct _q0 as [blk ofs].
@@ -35,9 +37,9 @@ Module IncrementIA. Section IncrementIA.
 
     sch_yield_l. steps_l. rename _q into v.
 
-    steps_r. inline_r. unfold_lat_real_r. force_r (blk, ofs, 1%Qp, Vint v).
-    iFrame. iSplit; et.
-    iIntros "[PT ->]". steps_r. hss_r. steps_r.
+    steps_r. inline_r. force_r (blk, ofs, 1%Qp, Vint v). steps_r.
+    forces_r. iFrame "ASM". iSplit; eauto.
+    steps_r. iDestruct "GRT" as "[[PT ->] ->]". hss_r. steps_r.
 
     force_l false. steps_l. force_l; iFrame "PT". steps_l. sch_yield_l. steps_l.
     unfold_iterC_l. steps_l.
@@ -46,11 +48,12 @@ Module IncrementIA. Section IncrementIA.
     sch_yield_rr. steps_r.
 
     sch_yield_l. steps_l. rename _q into v'.
-    inline_r. unfold_lat_real_r. force_r (_, _, _, _, _, _, _, _, _, _).
-    iSplitL "ASM".
-    { s. iFrame. repeat (iSplit; eauto). s. des_ifs. }
-    iIntros "[-> [GRT _]]". steps_r. hss. steps_r.
+    inline_r. force_r (_, _, _, _, _, _, _, _, _, _). forces_r. iFrame "ASM".
+    iSplitL ""; eauto.
+    { iSplit; eauto. iSplit; [iPureIntro; split; [refl|ss]|ss]. des_ifs. }
+    Unshelve. all: try exact 0; try exact 1%Qp; try exact (Vint 0).
 
+    steps_r. iDestruct "GRT" as "[[-> [GRT _]] ->]". hss_r. steps_r.
     destruct (dec v' v) as [?|Heq]; [subst; ss|ss].
     { force_l true. steps_l. force_l; iFrame "GRT"; steps_l.
       sch_yield_rr. steps_r.
@@ -69,6 +72,6 @@ Module IncrementIA. Section IncrementIA.
       iApply wsim_progress. iApply wsim_base.
       iIntros "?". iApply (CIH). iFrame.
     }
-    Unshelve. all: eauto. all: try exact 1%Qp. all: try exact Vundef.
+    Unshelve. all: eauto.
   (*SLOW*)Qed.
 End IncrementIA. End IncrementIA.
