incr_faa/FaaIA.v
@@ -3,14 +3,16 @@ From CRIS.incr_faa Require Import Header FaaI FaaA.
 Require Import ImpPrelude MemHeader MemA SchA SchTactics SchHeader.
 
 Module FaaIA. Section FaaIA.
-  Context `{!crisG Γ Σ α β τ _S _I, !memG, !schG}.
+  Context `{CrisG: !crisG Γ Σ α β τ _S _I}.
+  Context `{MemG: !memG}.
+  Context `{SchG: !schG}.
 
   Local Definition IstFull := (IstProd (IstSB FaaA.t.(Mod.scopes) IstTrue) IstEq).
-  Local Definition MA := (FaaA.t ★ MemP.t).
-  Local Definition MI := (FaaI.t ★ MemP.t).
+  Local Definition MA := (FaaA.t ★ MemA.t).
+  Local Definition MI := (FaaI.t ★ MemA.t).
 
   Lemma faa2_simF : ISim.sim_fun open MA MI True%I IstFull (Some FaaHdr.faa2).
-  Proof.
+  Proof using MemG SchG.
     init_simF.
 
     steps_l.
@@ -23,27 +25,23 @@ Module FaaIA. Section FaaIA.
     sch_yield_l; steps_l. rename _q into v.
 
     rewrite /MemHdr.faa; steps_r; inline_r.
-    unfold_lat_real_r. force_r (_, _, _, Vint v).
-    iFrame "ASM". iSplit; et.
-    iIntros "[PT ->]". steps_r. hss_r. steps_r.
-    
-    inline_r.
-    unfold_lat_real_r. force_r (_, _, _, _).
-    iFrame "PT". iSplit; et.
-    iIntros "[PT ->]". steps_r. hss_r. steps_r.
+    force_r (_, _, _, Vint v); forces_r; iFrame "ASM"; iSplit; eauto.
+    steps_r; iDestruct "GRT" as "[[PT ->] ->]"; hss_r.
+    steps_r; inline_r.
+    force_r (_, _, _, _); forces_r; iFrame "PT"; iSplit; eauto.
+    steps_r; iDestruct "GRT" as "[[PT ->] ->]"; hss_r. steps_r.
 
     force_l; iFrame "PT"; steps_l.
+
     sch_yield_rr.
     Unshelve. all: try exact 0.
     sch_yield_l; steps_l; clear v; rename _q into v.
     steps_r; inline_r.
-    unfold_lat_real_r. force_r (_, _, _, _).
-    iFrame. iSplit; et.
-    iIntros "[PT ->]". steps_r. hss_r. steps_r.
+    force_r (_, _, _, _); forces_r; iFrame "ASM"; iSplit; eauto.
+    steps_r; iDestruct "GRT" as "[[PT ->] ->]"; hss_r.
     steps_r; inline_r.
-    unfold_lat_real_r. force_r (_, _, _, _).
-    iFrame. iSplit; et.
-    iIntros "[PT ->]". steps_r. hss_r. steps_r.
+    force_r (_, _, _, _); forces_r; iFrame "PT"; iSplit; eauto.
+    steps_r; iDestruct "GRT" as "[[PT ->] ->]"; hss_r.
 
     force_l; iFrame "PT"; steps_l.
     steps_r.
@@ -56,7 +54,7 @@ Module FaaIA. Section FaaIA.
   (*SLOW*)Qed.
 
   Lemma sim : ISim.t open MA MI emp%I IstFull.
-  Proof.
+  Proof using MemG SchG.
     init_sim.
     { split; ss; iIntros "_"; iSplit; eauto. }
     { eapply faa2_simF. }
